Remove footprint.

pulse/lib/pulse/lib/Pulse.Lib.ArrayPtr.fst
@@ -23,54 +23,44 @@ type ptr t = {
     offset: (offset: SZ.t { SZ.v offset <= A.length base})
 }
 
-[@@erasable]
-noeq
-type footprint (t: Type0) = {
-    elt: ptr t;
-    len: (len: SZ.t { SZ.v elt.offset + SZ.v len <= A.length elt.base});
-}
+let base a = a.base
+let offset a = SZ.v a.offset
 
-let pts_to s #p fp v =
-    A.pts_to_range s.base (SZ.v s.offset) (SZ.v s.offset + SZ.v fp.len) #p v **
-    pure (fp.elt == s)
+let pts_to s #p v =
+    A.pts_to_range s.base (SZ.v s.offset) (SZ.v s.offset + Seq.length v) #p v
 
-let pts_to_is_slprop2 x p fp s = ()
+let pts_to_is_slprop2 x p s = ()
 
-let is_from_array p fp a =
-    pure (fp.elt.base == a /\ SZ.v fp.len == A.length a)
+let is_from_array s sz a =
+    pure (sz == A.length a /\ s.base == a)
 
 fn from_array (#t: Type) (a: A.array t) (#p: perm) (#v: Ghost.erased (Seq.seq t))
     requires A.pts_to a #p v
     returns s: ptr t
-    ensures exists* fp . pts_to s #p fp v ** is_from_array p fp a
+    ensures pts_to s #p v ** is_from_array s (Seq.length v) a
 {
     A.pts_to_len a;
     let res = {
         base = a;
         offset = 0sz;
     };
-    let fp = {
-        elt = res;
-        len = SZ.uint_to_t (A.length a);
-    };
-    fold (is_from_array p fp a);
+    fold (is_from_array res (Seq.length v) a);
     A.pts_to_range_intro a p v;
     rewrite (A.pts_to_range a 0 (A.length a) #p v)
-        as (A.pts_to_range res.base (SZ.v res.offset) (SZ.v res.offset + SZ.v fp.len) #p v);
-    fold (pts_to res #p fp v);
+        as (A.pts_to_range res.base (SZ.v res.offset) (SZ.v res.offset + Seq.length v) #p v);
+    fold (pts_to res #p v);
     res
 }
 
 ghost
-fn to_array (#t: Type) (s: ptr t) (a: array t) (#p: perm) (#fp: footprint t) (#v: Seq.seq t)
-    requires pts_to s #p fp v ** is_from_array p fp a ** pure (
-        Seq.length v == A.length a
-    )
+fn to_array (#t: Type) (s: ptr t) (a: array t) (#p: perm) (#v: Seq.seq t)
+    requires pts_to s #p v ** is_from_array s (Seq.length v) a
     ensures A.pts_to a #p v
 {
-    unfold (is_from_array p fp a);
-    unfold (pts_to s #p fp v);
-    rewrite (A.pts_to_range s.base (SZ.v s.offset) (SZ.v s.offset + SZ.v fp.len) #p v)
+    unfold is_from_array s (Seq.length v) a;
+    unfold pts_to s #p v;
+    A.pts_to_range_prop s.base;
+    rewrite (A.pts_to_range s.base (SZ.v s.offset) (SZ.v s.offset + Seq.length v) #p v)
         as (A.pts_to_range a 0 (A.length a) #p v);
     A.pts_to_range_elim a _ _;
 }
@@ -80,21 +70,20 @@ fn op_Array_Access
         (a: ptr t)
         (i: SZ.t)
         (#p: perm)
-        (#fp: footprint t)
         (#s: Ghost.erased (Seq.seq t))
    requires
-     pts_to a #p fp s ** pure (SZ.v i < Seq.length s)
+     pts_to a #p s ** pure (SZ.v i < Seq.length s)
    returns res: t
    ensures
-            pts_to a #p fp s **
+            pts_to a #p s **
             pure (
               SZ.v i < Seq.length s /\
               res == Seq.index s (SZ.v i))
 {
-    unfold (pts_to a #p fp s);
+    unfold pts_to a #p s;
     A.pts_to_range_prop a.base;
     let res = A.pts_to_range_index a.base (SZ.add a.offset i);
-    fold (pts_to a #p fp s);
+    fold pts_to a #p s;
     res
 }
 
@@ -103,20 +92,19 @@ fn op_Array_Assignment
         (a: ptr t)
         (i: SZ.t)
         (v: t)
-        (#fp: footprint t)
         (#s: Ghost.erased (Seq.seq t))
    requires
-     pts_to a fp s ** pure (SZ.v i < Seq.length s)
+     pts_to a s ** pure (SZ.v i < Seq.length s)
    ensures exists* s' .
-            pts_to a fp s' **
+            pts_to a s' **
             pure (SZ.v i < Seq.length s /\
               s' == Seq.upd s (SZ.v i) v
             )
 {
-    unfold (pts_to a fp s);
+    unfold pts_to a s;
     A.pts_to_range_prop a.base;
     let res = A.pts_to_range_upd a.base (SZ.add a.offset i) v;
-    fold (pts_to a fp (Seq.upd s (SZ.v i) v));
+    fold pts_to a (Seq.upd s (SZ.v i) v);
 }
 
 ghost
@@ -124,15 +112,14 @@ fn share
   (#a:Type)
   (arr:ptr a)
   (#s:Ghost.erased (Seq.seq a))
-  (#fp: footprint a)
   (#p:perm)
-    requires pts_to arr #p fp s
-    ensures pts_to arr #(p /. 2.0R) fp s ** pts_to arr #(p /. 2.0R) fp s
+  requires pts_to arr #p s
+  ensures pts_to arr #(p /. 2.0R) s ** pts_to arr #(p /. 2.0R) s
 {
-    unfold (pts_to arr #p fp s);
+    unfold pts_to arr #p s;
     A.pts_to_range_share arr.base;
-    fold (pts_to arr #(p /. 2.0R) fp s);
-    fold (pts_to arr #(p /. 2.0R) fp s);    
+    fold pts_to arr #(p /. 2.0R) s;
+    fold pts_to arr #(p /. 2.0R) s;    
 }
 
 ghost
@@ -141,98 +128,77 @@ fn gather
   (arr:ptr a)
   (#s0 #s1:Ghost.erased (Seq.seq a))
   (#p0 #p1:perm)
-  (#fp: footprint a)
-      requires pts_to arr #p0 fp s0 ** pts_to arr #p1 fp s1
-      ensures pts_to arr #(p0 +. p1) fp s0 ** pure (s0 == s1)
+  requires pts_to arr #p0 s0 ** pts_to arr #p1 s1 ** pure (Seq.length s0 == Seq.length s1)
+  ensures pts_to arr #(p0 +. p1) s0 ** pure (s0 == s1)
 {
-    unfold (pts_to arr #p0 fp s0);
-    unfold (pts_to arr #p1 fp s1);
+    unfold pts_to arr #p0 s0;
+    unfold pts_to arr #p1 s1;
     A.pts_to_range_gather arr.base;
-    fold (pts_to arr #(p0 +. p1) fp s0)
+    fold pts_to arr #(p0 +. p1) s0
 }
 
-let adjacent fp1 fp2 =
-    fp1.elt.base == fp2.elt.base /\
-    SZ.v fp1.elt.offset + SZ.v fp1.len == SZ.v fp2.elt.offset
-
-let merge fp1 fp2 = {
-    elt = fp1.elt;
-    len = SZ.add fp1.len fp2.len;
-}
-
-let merge_assoc fp1 fp2 fp3 = ()
-
-fn split (#t: Type) (s: ptr t) (#p: perm) (#fp: footprint t) (#v: Ghost.erased (Seq.seq t)) (i: SZ.t)
-    requires pts_to s #p fp v ** pure (SZ.v i <= Seq.length v)
-    returns s' : ptr t
-    ensures
-        exists* v1 v2 fp1 fp2 .
-            pts_to s #p fp1 v1 **
-            pts_to s' #p fp2 v2 **
-            pure (split_postcond fp v i v1 v2 fp1 fp2)
+fn split (#t: Type) (s: ptr t) (#p: perm) (#v: Ghost.erased (Seq.seq t)) (i: SZ.t { SZ.v i <= Seq.length v })
+  requires pts_to s #p v
+  returns s' : ptr t
+  ensures
+    pts_to s #p (Seq.slice v 0 (SZ.v i)) **
+    pts_to s' #p (Seq.slice v (SZ.v i) (Seq.length v)) **
+    pure (adjacent s (SZ.v i) s')
 {
-    unfold (pts_to s #p fp v);
+    unfold pts_to s #p v;
     A.pts_to_range_prop s.base;
     let s' = {
         base = s.base;
         offset = SZ.add s.offset i;
     };
-    let fp1 = {
-        elt = fp.elt;
-        len = i;
-    };
-    let fp2 = {
-        elt = s';
-        len = SZ.sub fp.len i;
-    };
     A.pts_to_range_split s.base _ (SZ.v s'.offset) _;
-    with s1 . assert (A.pts_to_range s.base (SZ.v s.offset) (SZ.v s'.offset) #p s1);
+    with s1. assert A.pts_to_range s.base (SZ.v s.offset) (SZ.v s'.offset) #p s1;
     rewrite
         (A.pts_to_range s.base (SZ.v s.offset) (SZ.v s'.offset) #p s1)
-        as (A.pts_to_range s.base (SZ.v s.offset) (SZ.v s.offset + SZ.v fp1.len) #p s1);
-    fold (pts_to s #p fp1 s1);
-    with s2 . assert (A.pts_to_range s.base (SZ.v s'.offset) (SZ.v s.offset + SZ.v fp.len) #p s2);
+        as (A.pts_to_range s.base (SZ.v s.offset) (SZ.v s.offset + SZ.v i) #p s1);
+    fold pts_to s #p s1;  
+    with s2. assert A.pts_to_range s.base (SZ.v s'.offset) (SZ.v s.offset + Seq.length v) #p s2;
     rewrite
-        (A.pts_to_range s.base (SZ.v s'.offset) (SZ.v s.offset + SZ.v fp.len) #p s2)
-        as (A.pts_to_range s'.base (SZ.v s'.offset) (SZ.v s'.offset + SZ.v fp2.len) #p s2);
-    fold (pts_to s' #p fp2 s2);
+        (A.pts_to_range s.base (SZ.v s'.offset) (SZ.v s.offset + Seq.length v) #p s2)
+        as (A.pts_to_range s'.base (SZ.v s'.offset) (SZ.v s'.offset + Seq.length s2) #p s2);
+    fold pts_to s' #p s2;
     s'
 }
 
 ghost
-fn join (#t: Type) (s1: ptr t) (#p: perm) (#fp1: footprint t) (#v1: Seq.seq t) (s2: ptr t) (#fp2: footprint t {adjacent fp1 fp2}) (#v2: Seq.seq t)
-    requires pts_to s1 #p fp1 v1 ** pts_to s2 #p fp2 v2
-    ensures pts_to s1 #p (merge fp1 fp2) (Seq.append v1 v2)
+fn join (#t: Type) (s1: ptr t) (#p: perm) (#v1: Seq.seq t) (s2: ptr t) (#v2: Seq.seq t)
+    requires pts_to s1 #p v1 ** pts_to s2 #p v2 ** pure (adjacent s1 (Seq.length v1) s2)
+    ensures pts_to s1 #p (Seq.append v1 v2)
 {
-    unfold (pts_to s1 #p fp1 v1);
-    unfold (pts_to s2 #p fp2 v2);
-    rewrite (A.pts_to_range s2.base (SZ.v s2.offset) (SZ.v s2.offset + SZ.v fp2.len) #p v2)
-        as (A.pts_to_range s1.base (SZ.v s1.offset + SZ.v fp1.len) (SZ.v s1.offset + SZ.v (merge fp1 fp2).len) #p v2);
-    A.pts_to_range_join s1.base (SZ.v s1.offset) (SZ.v s1.offset + SZ.v fp1.len) (SZ.v s1.offset + SZ.v (merge fp1 fp2).len);
-    fold (pts_to s1 #p (merge fp1 fp2) (Seq.append v1 v2))
+    unfold pts_to s1 #p v1;
+    unfold pts_to s2 #p v2;
+    rewrite (A.pts_to_range s2.base (SZ.v s2.offset) (SZ.v s2.offset + Seq.length v2) #p v2)
+        as (A.pts_to_range s1.base (SZ.v s1.offset + Seq.length v1) (SZ.v s1.offset + Seq.length v1 + Seq.length v2) #p v2);
+    A.pts_to_range_join s1.base (SZ.v s1.offset) (SZ.v s1.offset + Seq.length v1) (SZ.v s1.offset + Seq.length v1 + Seq.length v2);
+    fold (pts_to s1 #p (Seq.append v1 v2))
 }
 
 module R = Pulse.Lib.Reference
 
-fn blit (#t:_) (#p0:perm) (#s0 #s1:Ghost.erased (Seq.seq t)) (#fp0 #fp1: footprint t)
+fn blit (#t:_) (#p0:perm) (#s0 #s1:Ghost.erased (Seq.seq t))
            (src:ptr t)
            (idx_src: SZ.t)
            (dst:ptr t)
            (idx_dst: SZ.t)
            (len: SZ.t)
 requires
-    (pts_to src #p0 fp0 s0 ** pts_to dst fp1 s1 ** pure (
+    (pts_to src #p0 s0 ** pts_to dst s1 ** pure (
       SZ.v idx_src + SZ.v len <= Seq.length s0 /\
       SZ.v idx_dst + SZ.v len <= Seq.length s1
     ))
 ensures
-    (exists* s1' . pts_to src #p0 fp0 s0 ** pts_to dst fp1 s1' **
+    (exists* s1' . pts_to src #p0 s0 ** pts_to dst s1' **
       pure (blit_post s0 s1 idx_src idx_dst len s1')
     )
 {
-  unfold (pts_to src #p0 fp0 s0);
+  unfold (pts_to src #p0 s0);
   A.pts_to_range_prop src.base;
-  fold (pts_to src #p0 fp0 s0);
+  fold (pts_to src #p0 s0);
   let mut pi = 0sz;
   while (
     let i = !pi;
@@ -240,18 +206,18 @@ ensures
   )
   invariant b . exists* i s1' .
     R.pts_to pi i **
-    pts_to src #p0 fp0 s0 **
-    pts_to dst fp1 s1' **
+    pts_to src #p0 s0 **
+    pts_to dst s1' **
     pure (
       SZ.v i <= SZ.v len /\
       b == (SZ.v i < SZ.v len) /\
       blit_post s0 s1 idx_src idx_dst i s1'
     )
   {
-    with s1' . assert (pts_to dst fp1 s1');
-    unfold (pts_to dst fp1 s1');
+    with s1'. assert pts_to dst s1';
+    unfold pts_to dst s1';
     A.pts_to_range_prop dst.base;
-    fold (pts_to dst fp1 s1');
+    fold pts_to dst s1';
     let i = !pi;
     let x = op_Array_Access src (SZ.add idx_src i);
     op_Array_Assignment dst (SZ.add idx_dst i) x;
@@ -259,7 +225,7 @@ ensures
     Seq.lemma_split (Seq.slice s1' (SZ.v idx_dst) (SZ.v idx_dst + SZ.v (SZ.add i 1sz))) (SZ.v i);
     Seq.lemma_split (Seq.slice s0 (SZ.v idx_src) (SZ.v idx_src + SZ.v (SZ.add i 1sz))) (SZ.v i);
     Seq.slice_slice s1' (SZ.v idx_dst + SZ.v i) (Seq.length s1') 1 (Seq.length s1' - (SZ.v idx_dst + SZ.v i));
-    with s1'' . assert (pts_to dst fp1 s1'');
+    with s1''. assert pts_to dst s1'';
     assert (pure (
         Seq.slice s1'' (SZ.v idx_dst + SZ.v (SZ.add i 1sz)) (Seq.length s1) `Seq.equal`
           Seq.slice s1' (SZ.v idx_dst + SZ.v (SZ.add i 1sz)) (Seq.length s1')
