pulse/lib/pulse/lib/Pulse.Lib.ArrayPtr.fsti
@@ -24,25 +24,23 @@ module A = Pulse.Lib.Array
 
 val ptr : Type0 -> Type0
 
-[@@erasable]
-val footprint : Type0 -> Type0
+val base #t (p: ptr t) : GTot (A.array t)
+val offset #t (p: ptr t) : GTot nat
 
-val pts_to (#t: Type) (s: ptr t) (#[exact (`1.0R)] p: perm) (fp: footprint t) (v: Seq.seq t) : slprop
+val pts_to (#t: Type) (s: ptr t) (#[exact (`1.0R)] p: perm) (v: Seq.seq t) : slprop
 
-val pts_to_is_slprop2 (#a:Type) (x:ptr a) (p:perm) (fp: footprint a) (s:Seq.seq a)
-  : Lemma (is_slprop2 (pts_to x #p fp s))
-          [SMTPat (is_slprop2 (pts_to x #p fp s))]
+val pts_to_is_slprop2 (#a:Type) (x:ptr a) (p:perm) (s:Seq.seq a)
+  : Lemma (is_slprop2 (pts_to x #p s))
+          [SMTPat (is_slprop2 (pts_to x #p s))]
 
-val is_from_array (#t: Type) (p: perm) (fp: footprint t) (a: A.array t) : slprop
+val is_from_array (#t: Type) (s: ptr t) (sz: nat) (a: A.array t) : slprop
 
 val from_array (#t: Type) (a: A.array t) (#p: perm) (#v: Ghost.erased (Seq.seq t)) : stt (ptr t)
     (A.pts_to a #p v)
-    (fun s -> exists* fp . pts_to s #p fp v ** is_from_array p fp a)
+    (fun s -> pts_to s #p v ** is_from_array s (Seq.length v) a)
 
-val to_array (#t: Type) (s: ptr t) (a: array t) (#p: perm) (#fp: footprint t) (#v: Seq.seq t) : stt_ghost unit emp_inames
-    (pts_to s #p fp v ** is_from_array p fp a ** pure (
-        Seq.length v == A.length a
-    ))
+val to_array (#t: Type) (s: ptr t) (a: array t) (#p: perm) (#v: Seq.seq t) : stt_ghost unit emp_inames
+    (pts_to s #p v ** is_from_array s (Seq.length v) a)
     (fun _ -> A.pts_to a #p v)
 
 (* Written x.(i) *)
@@ -51,13 +49,12 @@ val op_Array_Access
         (a: ptr t)
         (i: SZ.t)
         (#p: perm)
-        (#fp: footprint t)
         (#s: Ghost.erased (Seq.seq t))
   : stt t
         (requires
-            pts_to a #p fp s ** pure (SZ.v i < Seq.length s))
+            pts_to a #p s ** pure (SZ.v i < Seq.length s))
         (ensures fun res ->
-            pts_to a #p fp s **
+            pts_to a #p s **
             pure (
               SZ.v i < Seq.length s /\
               res == Seq.index s (SZ.v i)))
@@ -68,13 +65,12 @@ val op_Array_Assignment
         (a: ptr t)
         (i: SZ.t)
         (v: t)
-        (#fp: footprint t)
         (#s: Ghost.erased (Seq.seq t))
   : stt unit
         (requires
-            pts_to a fp s ** pure (SZ.v i < Seq.length s))
+            pts_to a s ** pure (SZ.v i < Seq.length s))
         (ensures fun res -> exists* s' .
-            pts_to a fp s' **
+            pts_to a s' **
             pure (SZ.v i < Seq.length s /\
               s' == Seq.upd s (SZ.v i) v
             ))
@@ -83,11 +79,10 @@ val share
   (#a:Type)
   (arr:ptr a)
   (#s:Ghost.erased (Seq.seq a))
-  (#fp: footprint a)
   (#p:perm)
 : stt_ghost unit emp_inames
-      (requires pts_to arr #p fp s)
-      (ensures fun _ -> pts_to arr #(p /. 2.0R) fp s ** pts_to arr #(p /. 2.0R) fp s)
+      (requires pts_to arr #p s)
+      (ensures fun _ -> pts_to arr #(p /. 2.0R) s ** pts_to arr #(p /. 2.0R) s)
 
 [@@allow_ambiguous]
 val gather
@@ -95,51 +90,25 @@ val gather
   (arr:ptr a)
   (#s0 #s1:Ghost.erased (Seq.seq a))
   (#p0 #p1:perm)
-  (#fp: footprint a)
 : stt_ghost unit emp_inames
-      (requires pts_to arr #p0 fp s0 ** pts_to arr #p1 fp s1)
-      (ensures fun _ -> pts_to arr #(p0 +. p1) fp s0 ** pure (s0 == s1))
+      (requires pts_to arr #p0 s0 ** pts_to arr #p1 s1 ** pure (Seq.length s0 == Seq.length s1))
+      (ensures fun _ -> pts_to arr #(p0 +. p1) s0 ** pure (s0 == s1))
 
-val adjacent (#t: Type): footprint t -> footprint t -> prop
 
-val merge (#t: Type): (fp1: footprint t) -> (fp2: footprint t {adjacent fp1 fp2}) -> footprint t
+let adjacent #t (a: ptr t) (sz: nat) (b: ptr t) : prop =
+  base a == base b /\ offset a + sz == offset b
 
-val merge_assoc (#t: Type): (fp1: footprint t) -> (fp2: footprint t) -> (fp3: footprint t) -> Lemma
-    (ensures (
-        ((adjacent fp1 fp2 /\ adjacent (merge fp1 fp2) fp3) <==> (adjacent fp1 fp2 /\ adjacent fp2 fp3)) /\
-        ((adjacent fp2 fp3 /\ adjacent fp1 (merge fp2 fp3)) <==> (adjacent fp1 fp2 /\ adjacent fp2 fp3)) /\
-        ((adjacent fp1 fp2 /\ adjacent fp2 fp3) ==> 
-            merge (merge fp1 fp2) fp3 == merge fp1 (merge fp2 fp3)
-        )
-    ))
-    [SMTPatOr [
-        [SMTPat (adjacent fp1 fp2); SMTPat (adjacent (merge fp1 fp2) fp3)];
-        [SMTPat (adjacent fp2 fp3); SMTPat (adjacent fp1 (merge fp2 fp3))];
-        [SMTPat (adjacent fp1 fp2); SMTPat (adjacent fp2 fp3)];
-    ]]
-
-let split_postcond
-    (#t: Type) (fp: footprint t) (v: Ghost.erased (Seq.seq t)) (i: SZ.t)
-    (v1: Seq.seq t) (v2: Seq.seq t) (fp1: footprint t) (fp2: footprint t)
-: Tot prop
-=
-                adjacent fp1 fp2 /\
-                merge fp1 fp2 == fp /\
-                SZ.v i <= Seq.length v /\
-                (v1, v2) == Seq.split v (SZ.v i)
-
-val split (#t: Type) (s: ptr t) (#p: perm) (#fp: footprint t) (#v: Ghost.erased (Seq.seq t)) (i: SZ.t) : stt (ptr t)
-    (requires pts_to s #p fp v ** pure (SZ.v i <= Seq.length v))
+val split (#t: Type) (s: ptr t) (#p: perm) (#v: Ghost.erased (Seq.seq t)) (i: SZ.t { SZ.v i <= Seq.length v }) : stt (ptr t)
+    (requires pts_to s #p v)
     (ensures fun s' ->
-        exists* v1 v2 fp1 fp2 .
-            pts_to s #p fp1 v1 **
-            pts_to s' #p fp2 v2 **
-            pure (split_postcond fp v i v1 v2 fp1 fp2)
+        pts_to s #p (Seq.slice v 0 (SZ.v i)) **
+        pts_to s' #p (Seq.slice v (SZ.v i) (Seq.length v)) **
+        pure (adjacent s (SZ.v i) s')
     )
 
-val join (#t: Type) (s1: ptr t) (#p: perm) (#fp1: footprint t) (#v1: Seq.seq t) (s2: ptr t) (#fp2: footprint t {adjacent fp1 fp2}) (#v2: Seq.seq t) : stt_ghost unit emp_inames
-    (pts_to s1 #p fp1 v1 ** pts_to s2 #p fp2 v2)
-    (fun _ -> pts_to s1 #p (merge fp1 fp2) (Seq.append v1 v2))
+val join (#t: Type) (s1: ptr t) (#p: perm) (#v1: Seq.seq t) (s2: ptr t) (#v2: Seq.seq t) : stt_ghost unit emp_inames
+    (pts_to s1 #p v1 ** pts_to s2 #p v2 ** pure (adjacent s1 (Seq.length v1) s2))
+    (fun _ -> pts_to s1 #p (Seq.append v1 v2))
 
 let blit_post
 (#t:_) (s0 s1:Ghost.erased (Seq.seq t))
@@ -159,17 +128,17 @@ let blit_post
         Seq.slice s1' (SZ.v idx_dst + SZ.v len) (Seq.length s1) `Seq.equal`
           Seq.slice s1 (SZ.v idx_dst + SZ.v len) (Seq.length s1)
 
-val blit (#t:_) (#p0:perm) (#s0 #s1:Ghost.erased (Seq.seq t)) (#fp0 #fp1: footprint t)
+val blit (#t:_) (#p0:perm) (#s0 #s1:Ghost.erased (Seq.seq t))
            (src:ptr t)
            (idx_src: SZ.t)
            (dst:ptr t)
            (idx_dst: SZ.t)
            (len: SZ.t)
   : stt unit
-    (pts_to src #p0 fp0 s0 ** pts_to dst fp1 s1 ** pure (
+    (pts_to src #p0 s0 ** pts_to dst s1 ** pure (
       SZ.v idx_src + SZ.v len <= Seq.length s0 /\
       SZ.v idx_dst + SZ.v len <= Seq.length s1
     ))
-    (fun _ -> exists* s1' . pts_to src #p0 fp0 s0 ** pts_to dst fp1 s1' **
+    (fun _ -> exists* s1' . pts_to src #p0 s0 ** pts_to dst s1' **
       pure (blit_post s0 s1 idx_src idx_dst len s1')
     )
