pulse/lib/pulse/lib/Pulse.Lib.Slice.fst
@@ -23,65 +23,55 @@ noeq
 type slice t = {
     elt: AP.ptr t;
     len: SZ.t;
-    fp: AP.footprint t;
 }
 
 let len s = s.len
 
 let pts_to #t s #p v =
-    AP.pts_to s.elt #p s.fp v **
+    AP.pts_to s.elt #p v **
     pure (Seq.length v == SZ.v s.len)
 
 let pts_to_is_slprop2 x p v = ()
 
 ghost
 fn pts_to_len (#t: Type) (s: slice t) (#p: perm) (#v: Seq.seq t)
-requires    (pts_to s #p v)
-ensures    (pts_to s #p v ** pure (Seq.length v == SZ.v (len s)))
-
+  requires pts_to s #p v
+  ensures pts_to s #p v ** pure (Seq.length v == SZ.v (len s))
 {
     unfold (pts_to s #p v);
     fold (pts_to s #p v)
 }
 
-let is_from_array #t a p s =
-    AP.is_from_array p s.fp a **
-    pure (SZ.v s.len == A.length a)
+let is_from_array a s =
+  AP.is_from_array s.elt (SZ.v s.len) a
 
-fn from_array (#t: Type) (mutb: bool) (a: array t) (#p: perm) (#v: Ghost.erased (Seq.seq t)) (alen: SZ.t {
-    SZ.v alen == A.length a /\
-    (mutb == true ==> p == 1.0R)
-})
-requires    (A.pts_to a #p v)
-returns s: (slice t)
-ensures    (
-        pts_to s #p v **
-        is_from_array a p s
-    )
+fn from_array (#t: Type) (mutb: bool) (a: array t) (#p: perm) (#v: Ghost.erased (Seq.seq t))
+  (alen: SZ.t { SZ.v alen == A.length a /\ (mutb == true ==> p == 1.0R) })
+  requires A.pts_to a #p v
+  returns s: (slice t)
+  ensures 
+    pts_to s #p v **
+    is_from_array a s
 {
     A.pts_to_len a;
     let ptr = AP.from_array a;
-    with fp . assert (AP.pts_to ptr #p fp v ** AP.is_from_array p fp a);
     let res : slice t = {
         elt = ptr;
         len = alen;
-        fp = fp;
     };
-    rewrite (AP.pts_to ptr #p fp v) as (AP.pts_to res.elt #p res.fp v);
-    fold (pts_to res #p v);
-    rewrite (AP.is_from_array p fp a) as (AP.is_from_array p res.fp a);
-    fold (is_from_array a p res);
+    fold pts_to res #p v;
+    fold is_from_array a res;
     res
 }
 
 ghost
 fn to_array
     (#t: Type) (s: slice t) (#p: perm) (#v: Seq.seq t) (#a: array t)
-requires    (pts_to s #p v ** is_from_array a p s)
+requires    (pts_to s #p v ** is_from_array a s)
 ensures    (A.pts_to a #p v)
 {
     unfold (pts_to s #p v);
-    unfold (is_from_array a p s);
+    unfold is_from_array a s;
     AP.to_array s.elt a
 }
 
@@ -151,15 +141,14 @@ ensures pts_to arr #(p0 +. p1) s0 ** pure (s0 == s1)
     fold (pts_to arr #(p0 +. p1) s0)
 }
 
-let is_split #t s p i s1 s2 =
+let is_split #t s s1 s2 =
     pure (
         s1.elt == s.elt /\
-        AP.adjacent s1.fp s2.fp /\
-        AP.merge s1.fp s2.fp == s.fp /\
+        AP.adjacent s1.elt (SZ.v s1.len) s2.elt /\
         SZ.v s.len == SZ.v s1.len + SZ.v s2.len
     )
 
-let is_split_is_slprop2 s p i s1 s2 = ()
+let is_split_is_slprop2 s s1 s2 = ()
 
 fn split (#t: Type) (mutb: bool) (s: slice t) (#p: perm) (#v: Ghost.erased (Seq.seq t)) (i: SZ.t)
     requires pts_to s #p v ** pure (split_precond mutb p v i)
@@ -168,32 +157,30 @@ fn split (#t: Type) (mutb: bool) (s: slice t) (#p: perm) (#v: Ghost.erased (Seq.
 {
     unfold (pts_to s #p v);
     Seq.lemma_split v (SZ.v i);
-    let elt' = AP.split s.elt i;
-    with fp1 _v1 fp2 _v2 . assert (AP.pts_to s.elt #p fp1 _v1 ** AP.pts_to elt' #p fp2 _v2 ** pure (AP.split_postcond s.fp v i _v1 _v2 fp1 fp2));
+    let elt' = AP.split s.elt #p #v i;
+    with _v1 _v2. assert AP.pts_to s.elt #p _v1 ** AP.pts_to elt' #p _v2;
     let s1 = {
         elt = s.elt;
         len = i;
-        fp = fp1;
     };
     fold (pts_to s1 #p _v1);
     let s2 = {
         elt = elt';
         len = s.len `SZ.sub` i;
-        fp = fp2;
     };
     fold (pts_to s2 #p _v2);
-    fold (is_split s p i s1 s2);
+    fold (is_split s s1 s2);
     fold (split_post' s p v i s1 s2);
     fold (split_post s p v i (s1 `SlicePair` s2));
     (s1 `SlicePair` s2)
 }
 
 ghost
-fn join (#t: Type) (s1: slice t) (#p: perm) (#v1: Seq.seq t) (s2: slice t) (#v2: Seq.seq t) (#i: SZ.t) (s: slice t)
-    requires pts_to s1 #p v1 ** pts_to s2 #p v2 ** is_split s p i s1 s2
+fn join (#t: Type) (s1: slice t) (#p: perm) (#v1: Seq.seq t) (s2: slice t) (#v2: Seq.seq t) (s: slice t)
+    requires pts_to s1 #p v1 ** pts_to s2 #p v2 ** is_split s s1 s2
     ensures pts_to s #p (Seq.append v1 v2)
 {
-    unfold (is_split s p i s1 s2);
+    unfold (is_split s s1 s2);
     unfold (pts_to s1 #p v1);
     unfold (pts_to s2 #p v2);
     AP.join s1.elt s2.elt;
