pulse/lib/pulse/lib/Pulse.Lib.Slice.fsti
@@ -34,7 +34,7 @@ val pts_to_len (#t: Type) (s: slice t) (#p: perm) (#v: Seq.seq t) : stt_ghost un
     (pts_to s #p v)
     (fun _ -> pts_to s #p v ** pure (Seq.length v == SZ.v (len s)))
 
-val is_from_array (#t: Type) (a: array t) (p: perm) (s: slice t) : slprop
+val is_from_array (#t: Type) (a: array t) (s: slice t) : slprop
 
 val from_array (#t: Type) (mutb: bool) (a: array t) (#p: perm) (#v: Ghost.erased (Seq.seq t)) (alen: SZ.t {
     SZ.v alen == A.length a /\
@@ -43,11 +43,11 @@ val from_array (#t: Type) (mutb: bool) (a: array t) (#p: perm) (#v: Ghost.erased
     (A.pts_to a #p v)
     (fun s ->
         pts_to s #p v **
-        is_from_array a p s
+        is_from_array a s
     )
 
 val to_array (#t: Type) (s: slice t) (#p: perm) (#v: Seq.seq t) (#a: array t) : stt_ghost unit emp_inames
-    (pts_to s #p v ** is_from_array a p s)
+    (pts_to s #p v ** is_from_array a s)
     (fun _ -> A.pts_to a #p v)
 
 (* Written x.(i) *)
@@ -97,11 +97,11 @@ val gather
       (requires pts_to arr #p0 s0 ** pts_to arr #p1 s1)
       (ensures fun _ -> pts_to arr #(p0 +. p1) s0 ** pure (s0 == s1))
 
-val is_split (#t: Type) (s: slice t) (p: perm) (i: SZ.t) (left: slice t) (right: slice t) : slprop
+val is_split (#t: Type) (s: slice t) (left: slice t) (right: slice t) : slprop
 
-val is_split_is_slprop2 (#t: Type) (s: slice t) (p: perm) (i: SZ.t) (left: slice t) (right: slice t)
-  : Lemma (is_slprop2 (is_split s p i left right))
-          [SMTPat (is_slprop2 (is_split s p i left right))]
+val is_split_is_slprop2 (#t: Type) (s: slice t) (left: slice t) (right: slice t)
+  : Lemma (is_slprop2 (is_split s left right))
+          [SMTPat (is_slprop2 (is_split s left right))]
 
 noeq type slice_pair (t: Type) = | SlicePair: (fst: slice t) -> (snd: slice t) -> slice_pair t
 
@@ -118,7 +118,7 @@ let split_post'
 =       exists* v1 v2 .
             pts_to s1 #p v1 **
             pts_to s2 #p v2 **
-            is_split s p i s1 s2 **
+            is_split s s1 s2 **
             pure (
                 SZ.v i <= Seq.length v /\
                 (v1, v2) == Seq.split v (SZ.v i)
@@ -135,8 +135,8 @@ val split (#t: Type) (mutb: bool) (s: slice t) (#p: perm) (#v: Ghost.erased (Seq
     (requires pts_to s #p v ** pure (split_precond mutb p v i))
     (ensures fun res -> split_post s p v i res)
 
-val join (#t: Type) (s1: slice t) (#p: perm) (#v1: Seq.seq t) (s2: slice t) (#v2: Seq.seq t) (#i: SZ.t) (s: slice t) : stt_ghost unit emp_inames
-    (pts_to s1 #p v1 ** pts_to s2 #p v2 ** is_split s p i s1 s2)
+val join (#t: Type) (s1: slice t) (#p: perm) (#v1: Seq.seq t) (s2: slice t) (#v2: Seq.seq t) (s: slice t) : stt_ghost unit emp_inames
+    (pts_to s1 #p v1 ** pts_to s2 #p v2 ** is_split s s1 s2)
     (fun _ -> pts_to s #p (Seq.append v1 v2))
 
 val copy (#t: Type) (dst: slice t) (#p: perm) (src: slice t) (#v: Ghost.erased (Seq.seq t)) : stt unit
